Prove get_set_weak

examples/state.v
@@ -57,9 +57,11 @@ Qed.
 
 (* ========================================================================== *)
 
+Definition TyState := TyInt. (* Need some wellformed type *)
+
 Example sig := (SigU (SigU (SigØ) 
-    ("get") TyUnit TyInt)
-    ("set") TyInt TyUnit).
+    ("get") TyUnit TyState)
+    ("set") TyState TyUnit).
 
 
 Lemma wf_sig_sig:
@@ -82,7 +84,7 @@ Example state_cases := (CasesU (CasesU (CasesØ)
   
 Lemma has_htype_state_cases D :
   wf_ctype D ->
-  has_htype CtxØ state_cases sig (CTy (TyFun TyInt D) SigØ EqsØ).
+  has_htype CtxØ state_cases sig (CTy (TyFun TyState D) SigØ EqsØ).
 Proof.
 intros wfd.
 assert (wf_sig sig). apply wf_sig_sig. 
@@ -91,32 +93,32 @@ apply TypeH; obvious. apply TypeCasesU; obvious.
 apply TypeH; obvious. apply TypeCasesU; obvious.
 + apply TypeH; obvious. apply TypeCasesØ.
 + ctype_step. vtype_step.
-  eapply letbind_ctype. instantiate (1:=(TyFun TyInt D)).
-  ctype_step. instantiate (1:=TyInt). obvious_vtype. obvious_vtype.
-  ctype_step. instantiate (1:=TyInt). obvious_vtype. obvious_vtype.
+  eapply letbind_ctype. instantiate (1:=(TyFun TyState D)).
+  ctype_step. instantiate (1:=TyState). obvious_vtype. obvious_vtype.
+  ctype_step. instantiate (1:=TyState). obvious_vtype. obvious_vtype.
 + ctype_step. vtype_step.
-  eapply letbind_ctype. instantiate (1:=(TyFun TyInt D)).
+  eapply letbind_ctype. instantiate (1:=(TyFun TyState D)).
   ctype_step. instantiate (1:=TyUnit). obvious_vtype. obvious_vtype.
-  ctype_step. instantiate (1:=TyInt). obvious_vtype. obvious_vtype.
+  ctype_step. instantiate (1:=TyState). obvious_vtype. obvious_vtype.
 Qed.
 
 (* - - - - - - - - - - - - - - - - - - - - - - - - - - - - - - - - - - - - -  *)
 
 Example eq_set_set := (EqsU (EqsØ)
-  (CtxU (CtxU (CtxØ) TyInt) TyInt)
+  (CtxU (CtxU (CtxØ) TyState) TyState)
   (TCtxU (TCtxØ) TyUnit)
     (TOp "set" (Var 0) (TOp "set" (Var 2) (TApp 0 Unit)))
     (TOp "set" (Var 1) (TApp 0 Unit)) ).
 
 Example eq_get_get := (EqsU (EqsØ)
   CtxØ
-  (TCtxU (TCtxØ) (TyΠ TyInt TyInt))
+  (TCtxU (TCtxØ) (TyΠ TyState TyState))
     (TOp "get" Unit (TOp "get" Unit (TApp 0 (Pair (Var 0) (Var 1)))))
     (TOp "get" Unit (TApp 0 (Pair (Var 0) (Var 0)))) ).
 
 Example eq_set_get := (EqsU (EqsØ)
-  (CtxU (CtxØ) TyInt)
-  (TCtxU (TCtxØ) TyInt)
+  (CtxU (CtxØ) TyState)
+  (TCtxU (TCtxØ) TyState)
     (TOp "set" (Var 0) (TOp "get" Unit (TApp 0 (Var 0))))
     (TOp "set" (Var 0) (TApp 0 (Var 1))) ).
 
@@ -125,6 +127,12 @@ Example eq_get_set := (EqsU (EqsØ)
   (TCtxU (TCtxØ) TyUnit)
     (TOp "get" Unit (TOp "set" (Var 0) (TApp 0 Unit)))
     (TApp 0 Unit) ).
+
+Example eq_get_set_weak := (EqsU (EqsØ)
+  CtxØ
+  (TCtxU (TCtxØ) TyState)
+    (TOp "get" Unit (TOp "set" (Var 0) (TApp 0 (Var 1))))
+    (TOp "get" Unit (TApp 0 (Var 0))) ).
 
 Lemma wf_eq_set_set:
   wf_eqs eq_set_set sig.
@@ -174,13 +182,26 @@ apply WfEqsU; obvious.
 + eapply WfTApp. 2: simpl; reflexivity. obvious_vtype.
 Qed.
 
+
+Lemma wf_eq_get_set_weak:
+  wf_eqs eq_get_set_weak sig.
+Proof.
+unfold eq_get_set_weak. unfold sig.
+apply WfEqsU; obvious.
++ eapply WfTOp. simpl. reflexivity. obvious_vtype.
+  eapply WfTOp. simpl. reflexivity. obvious_vtype.
+  eapply WfTApp. 2: simpl; reflexivity. obvious_vtype.
++ eapply WfTOp. simpl. reflexivity. obvious_vtype.
+  eapply WfTApp. 2: simpl; reflexivity. obvious_vtype.
+Qed.
+
 (* ========================================================================== *)
 
 Lemma respects_set_set A:
   wf_vtype A ->
   respects
     CtxØ state_cases
-    sig (CTy (TyFun TyInt (CTy A SigØ EqsØ)) SigØ EqsØ) eq_set_set.
+    sig (CTy (TyFun TyState (CTy A SigØ EqsØ)) SigØ EqsØ) eq_set_set.
 Proof.
 intros wfa.
 unfold state_cases. unfold sig. unfold eq_set_set.
@@ -189,31 +210,31 @@ apply RespectEqsU. apply Respects; obvious. apply RespectEqsØ.
 simpl. simpl_c_subs. apply Ceq; obvious.
 
 { ctype_step. vtype_step. eapply letbind_ctype.
-  instantiate (1:=(TyFun TyInt (CTy A SigØ EqsØ))).
+  instantiate (1:=(TyFun TyState (CTy A SigØ EqsØ))).
   Focus 2. apply TypeC; obvious. eapply TypeApp.
-    instantiate (1:=TyInt). obvious_vtype. obvious_vtype.
+    instantiate (1:=TyState). obvious_vtype. obvious_vtype.
   ctype_step. 2: obvious_vtype. vtype_step. ctype_step. vtype_step.
-  eapply letbind_ctype. instantiate (1:= (TyFun TyInt (CTy A SigØ EqsØ))).
+  eapply letbind_ctype. instantiate (1:= (TyFun TyState (CTy A SigØ EqsØ))).
   + ctype_step. 2:obvious_vtype. vtype_step. obvious_ctype.
-  + ctype_step. instantiate (1:=TyInt). all: obvious_vtype. }
+  + ctype_step. instantiate (1:=TyState). all: obvious_vtype. }
 { ctype_step. vtype_step. eapply letbind_ctype.
-  instantiate (1:=(TyFun TyInt (CTy A SigØ EqsØ))).
-  Focus 2. ctype_step. instantiate (1:=TyInt). obvious_vtype. obvious_vtype.
+  instantiate (1:=(TyFun TyState (CTy A SigØ EqsØ))).
+  Focus 2. ctype_step. instantiate (1:=TyState). obvious_vtype. obvious_vtype.
   ctype_step. 2: obvious_vtype. vtype_step. obvious_ctype. }
 
 apply CeqRet. apply Veq; obvious.
 
 { vtype_step. eapply letbind_ctype.
-  instantiate (1:=(TyFun TyInt (CTy A SigØ EqsØ))).
+  instantiate (1:=(TyFun TyState (CTy A SigØ EqsØ))).
   Focus 2. apply TypeC; obvious. eapply TypeApp.
-    instantiate (1:=TyInt). obvious_vtype. obvious_vtype.
+    instantiate (1:=TyState). obvious_vtype. obvious_vtype.
   ctype_step. 2: obvious_vtype. vtype_step. ctype_step. vtype_step.
-  eapply letbind_ctype. instantiate (1:= (TyFun TyInt (CTy A SigØ EqsØ))).
+  eapply letbind_ctype. instantiate (1:= (TyFun TyState (CTy A SigØ EqsØ))).
   + ctype_step. 2:obvious_vtype. vtype_step. obvious_ctype.
-  + ctype_step. instantiate (1:=TyInt). all: obvious_vtype. }
+  + ctype_step. instantiate (1:=TyState). all: obvious_vtype. }
 { vtype_step. eapply letbind_ctype.
-  instantiate (1:=(TyFun TyInt (CTy A SigØ EqsØ))).
-  Focus 2. ctype_step. instantiate (1:=TyInt). obvious_vtype. obvious_vtype.
+  instantiate (1:=(TyFun TyState (CTy A SigØ EqsØ))).
+  Focus 2. ctype_step. instantiate (1:=TyState). obvious_vtype. obvious_vtype.
   ctype_step. 2: obvious_vtype. vtype_step. obvious_ctype. }
 
 apply VeqFun. eapply ceq_trans.
@@ -221,43 +242,43 @@ instantiate (1:=
   (DoBind (Ret (Fun
           (DoBind (App (Fun (App (Var 5) Unit)) Unit)
              (App (Var 0) (Var 4)))))) (App (Var 0) (Var 2)) ).
-eapply (letbind_reduce (TyFun TyInt (CTy A SigØ EqsØ))).
+eapply (letbind_reduce (TyFun TyState (CTy A SigØ EqsØ))).
 
 { apply Ceq; obvious. 3: apply βApp.
   { ctype_step. 2:obvious_vtype. vtype_step. ctype_step.
-    vtype_step. eapply (letbind_ctype (TyFun TyInt (CTy A SigØ EqsØ))).
+    vtype_step. eapply (letbind_ctype (TyFun TyState (CTy A SigØ EqsØ))).
     + ctype_step. 2:obvious_vtype. vtype_step. obvious_ctype.
-    + ctype_step. instantiate (1:=TyInt). all: obvious_vtype. }
-  { ctype_step. vtype_step. eapply (letbind_ctype (TyFun TyInt (CTy A SigØ EqsØ))).
+    + ctype_step. instantiate (1:=TyState). all: obvious_vtype. }
+  { ctype_step. vtype_step. eapply (letbind_ctype (TyFun TyState (CTy A SigØ EqsØ))).
     + ctype_step. 2:obvious_vtype. vtype_step. obvious_ctype.
-    + ctype_step. instantiate (1:=TyInt). all: obvious_vtype. } }
-{ ctype_step. instantiate (1:=TyInt). all: obvious_vtype. }
+    + ctype_step. instantiate (1:=TyState). all: obvious_vtype. } }
+{ ctype_step. instantiate (1:=TyState). all: obvious_vtype. }
 
 eapply ceq_trans. apply Ceq; obvious. 3: apply βDoBind_Ret.
 
-{ eapply letbind_ctype. instantiate (1:= (TyFun TyInt (CTy A SigØ EqsØ))).
-  ctype_step. vtype_step. eapply (letbind_ctype (TyFun TyInt (CTy A SigØ EqsØ))).
+{ eapply letbind_ctype. instantiate (1:= (TyFun TyState (CTy A SigØ EqsØ))).
+  ctype_step. vtype_step. eapply (letbind_ctype (TyFun TyState (CTy A SigØ EqsØ))).
   ctype_step. 2: obvious_vtype. vtype_step. obvious_ctype. 
-  ctype_step. instantiate (1:= TyInt). obvious_vtype. obvious_vtype.
-  ctype_step. instantiate (1:= TyInt). obvious_vtype. obvious_vtype. }
-{ simpl_c_subs. ctype_step. instantiate (1:= TyInt). 2:obvious_vtype.
-  vtype_step. eapply (letbind_ctype (TyFun TyInt (CTy A SigØ EqsØ))).
+  ctype_step. instantiate (1:= TyState). obvious_vtype. obvious_vtype.
+  ctype_step. instantiate (1:= TyState). obvious_vtype. obvious_vtype. }
+{ simpl_c_subs. ctype_step. instantiate (1:= TyState). 2:obvious_vtype.
+  vtype_step. eapply (letbind_ctype (TyFun TyState (CTy A SigØ EqsØ))).
   ctype_step. vtype_step. obvious_ctype. obvious_vtype.
-  ctype_step. instantiate (1:= TyInt). obvious_vtype. obvious_vtype. }
+  ctype_step. instantiate (1:= TyState). obvious_vtype. obvious_vtype. }
 
 simpl_c_subs. eapply ceq_trans. apply Ceq. 3: apply βApp. all: simpl_c_subs.
 
-{ ctype_step. instantiate (1:=TyInt). 2: obvious_vtype.
-  vtype_step.  eapply (letbind_ctype (TyFun TyInt (CTy A SigØ EqsØ))).
+{ ctype_step. instantiate (1:=TyState). 2: obvious_vtype.
+  vtype_step.  eapply (letbind_ctype (TyFun TyState (CTy A SigØ EqsØ))).
   ctype_step. vtype_step. obvious_ctype. obvious_vtype.
-  ctype_step. instantiate (1:= TyInt). obvious_vtype. obvious_vtype. }
-{ eapply (letbind_ctype (TyFun TyInt (CTy A SigØ EqsØ))).
+  ctype_step. instantiate (1:= TyState). obvious_vtype. obvious_vtype. }
+{ eapply (letbind_ctype (TyFun TyState (CTy A SigØ EqsØ))).
   ctype_step. vtype_step. obvious_ctype. obvious_vtype.
-  ctype_step. instantiate (1:= TyInt). obvious_vtype. obvious_vtype.  }
+  ctype_step. instantiate (1:= TyState). obvious_vtype. obvious_vtype.  }
 
-apply ceq_refl. eapply (letbind_ctype (TyFun TyInt (CTy A SigØ EqsØ))).
+apply ceq_refl. eapply (letbind_ctype (TyFun TyState (CTy A SigØ EqsØ))).
 ctype_step. vtype_step. obvious_ctype. obvious_vtype.
-ctype_step. instantiate (1:= TyInt). obvious_vtype. obvious_vtype.
+ctype_step. instantiate (1:= TyState). obvious_vtype. obvious_vtype.
 
 Qed.
 
@@ -267,7 +288,7 @@ Lemma respects_get_get A:
   wf_vtype A ->
   respects 
     CtxØ state_cases 
-    sig (CTy (TyFun TyInt (CTy A SigØ EqsØ)) SigØ EqsØ) eq_get_get.
+    sig (CTy (TyFun TyState (CTy A SigØ EqsØ)) SigØ EqsØ) eq_get_get.
 Proof.
 intros wfa.
 unfold state_cases. unfold sig. unfold eq_get_get.
@@ -293,7 +314,7 @@ simpl_c_subs. eapply ceq_trans. apply Ceq. 3: apply βApp.
 { admit. }
 { admit. }
 simpl_c_subs. apply Ceq. 3: eapply CeqDoBind. 
-3: instantiate (1:=(TyFun TyInt (CTy A SigØ EqsØ))).
+3: instantiate (1:=(TyFun TyState (CTy A SigØ EqsØ))).
 { admit. }
 { admit. }
 2: apply ceq_refl; admit.
@@ -314,7 +335,7 @@ Lemma respects_set_get A:
   wf_vtype A ->
   respects 
     CtxØ state_cases 
-    sig (CTy (TyFun TyInt (CTy A SigØ EqsØ)) SigØ EqsØ) eq_set_get.
+    sig (CTy (TyFun TyState (CTy A SigØ EqsØ)) SigØ EqsØ) eq_set_get.
 Proof.
 intros wfa.
 unfold state_cases. unfold sig. unfold eq_set_get.
@@ -340,7 +361,7 @@ simpl_c_subs. eapply ceq_trans. apply Ceq. 3: apply βApp.
 { admit. }
 { admit. }
 simpl_c_subs. apply Ceq. 3: eapply CeqDoBind. 
-3: instantiate (1:=(TyFun TyInt (CTy A SigØ EqsØ))).
+3: instantiate (1:=(TyFun TyState (CTy A SigØ EqsØ))).
 { admit. }
 { admit. }
 2: apply ceq_refl; admit.
@@ -361,7 +382,7 @@ Lemma respects_get_set A:
   wf_vtype A ->
   respects 
     CtxØ state_cases 
-    sig (CTy (TyFun TyInt (CTy A SigØ EqsØ)) SigØ EqsØ) eq_get_set.
+    sig (CTy (TyFun TyState (CTy A SigØ EqsØ)) SigØ EqsØ) eq_get_set.
 Proof.
 intros wfa.
 unfold state_cases. unfold sig. unfold eq_get_set.
@@ -369,4 +390,50 @@ apply Respects; obvious. apply wf_eq_get_set.
 apply RespectEqsU. apply Respects; obvious. apply RespectEqsØ.
 simpl. simpl_c_subs.
 admit.
+Admitted.
+
+(* - - - - - - - - - - - - - - - - - - - - - - - - - - - - - - - - - - - - -  *)
+
+Lemma respects_get_set_weak A:
+  wf_vtype A ->
+  respects 
+    CtxØ state_cases 
+    sig (CTy (TyFun TyState (CTy A SigØ EqsØ)) SigØ EqsØ) eq_get_set_weak.
+Proof.
+intros wfa.
+unfold state_cases. unfold sig. unfold eq_get_set_weak.
+apply Respects; obvious. apply wf_eq_get_set_weak.
+apply RespectEqsU. apply Respects; obvious. apply RespectEqsØ.
+simpl. simpl_c_subs.
+apply Ceq; obvious.
+{ admit. }
+{ admit. }
+apply CeqRet. apply Veq; obvious.
+{ admit. }
+{ admit. }
+apply VeqFun. eapply ceq_trans. apply Ceq. 3: eapply CeqDoBind.
+{ admit. }
+{ admit. }
+2: apply ceq_refl; admit. apply Ceq. 3: apply βApp.
+{ admit. }
+{ admit. }
+simpl_c_subs. eapply ceq_trans. apply Ceq. 3: apply βDoBind_Ret.
+{ admit. }
+{ admit. }
+simpl_c_subs. eapply ceq_trans. apply Ceq. 3: apply βApp.
+{ admit. }
+{ admit. }
+simpl_c_subs. apply Ceq. 3: eapply CeqDoBind. 
+3: instantiate (1:=(TyFun TyState (CTy A SigØ EqsØ))).
+{ admit. }
+{ admit. }
+2: apply ceq_refl; admit.
+eapply ceq_trans. apply Ceq. 3: eapply βApp.
+{ admit. }
+{ admit. }
+simpl_c_subs. apply ceq_sym.
+eapply ceq_trans. apply Ceq. 3: eapply βApp.
+{ admit. }
+{ admit. }
+simpl_c_subs. eapply ceq_refl. admit.
 Admitted.
